Proving Facade.v

platform/cito/facade/Facade.v
@@ -398,33 +398,87 @@ Module Make (Import A : ADT).
     edestruct IHRunsTo1; clear IHRunsTo1; eauto.
     Lemma safe_seq_1 : forall (env : Env) a b st, Safe env (Seq a b) st -> Safe env a st.
     Proof.
-      admit.
+      intros.
+      inversion H; subst.
+      openhyp.
+      eauto.
     Qed.
     eapply safe_seq_1; eauto.
     openhyp.
     edestruct IHRunsTo2; clear IHRunsTo2; eauto.
-    Lemma safe_seq_1 : forall (env : Env) a b st, Safe env (Seq a b) st -> Safe env a st.
+    Lemma safe_seq_2 : forall (env : Env) a b st, Safe env (Seq a b) st -> forall st', RunsTo env a st st' -> Safe env b st'.
     Proof.
-      admit.
+      intros.
+      inversion H; subst.
+      openhyp.
+      eauto.
     Qed.
+    eapply safe_seq_2; eauto.
+    openhyp.
+    eexists.
+    split.
+    eapply RunsToSeq; eauto.
+    eauto.
 
-
+    (* if-true *)
     injection H1; intros; subst; clear H1.
     edestruct IHRunsTo.
     eauto.
     eauto.
     eauto.
-    admit.
+    Notation ceval := SemanticsExpr.eval.
+    Notation cRunsTo := Semantics.RunsTo.
+    Lemma is_true_is_false : forall (st : State) e, is_true st e -> is_false st e -> False.
+    Proof.
+      intros.
+      unfold is_true, is_false in *.
+      rewrite H in *; discriminate.
+    Qed.
+    Lemma safe_if_true : forall (env : Env) e t f st, Safe env (If e t f) st -> is_true st e -> Safe env t st.
+    Proof.
+      intros.
+      inversion H; subst.
+      eauto.
+      exfalso.
+      eapply is_true_is_false; eauto.
+    Qed.
+    eapply safe_if_true; eauto.
+    Definition is_bool (st : State) e := eval_bool st e <> None.
+    Lemma wneb_is_true : forall s_st t_st e, wneb (ceval (fst t_st) e) $0 = true -> related_state s_st t_st -> is_bool s_st e -> is_true s_st e.
+    Proof.
+      intros.
+      unfold is_true.
+      unfold is_bool in *.
+      eapply ex_up in H1.
+      openhyp.
+      Notation boolcase := Sumbool.sumbool_of_bool.
+      destruct (boolcase x); subst.
+      eauto.
+      Lemma eval_bool_wneb : forall (s_st : State) t_st e b, eval_bool s_st e = Some b -> related_state s_st t_st -> wneb (ceval (fst t_st) e) $0 = b.
+      Proof.
+        admit.
+      Qed.
+      eapply eval_bool_wneb in H1; eauto.
+      set (ceval _ _) in *.
+      rewrite H in *; discriminate.
+    Qed.
+    eapply wneb_is_true; eauto.
+    Lemma safe_if_is_bool : forall (env : Env) e t f st, Safe env (If e t f) st -> is_bool st e.
+    Proof.
+      admit.
+    Qed.
+    eapply safe_if_is_bool; eauto.
     openhyp.
     eexists.
     split.
     eapply RunsToIfTrue.
-    unfold is_true.
-    unfold eval_bool.
-    admit.
+    eapply wneb_is_true; eauto.
+    eapply safe_if_is_bool; eauto.
 
     eauto.
     eauto.
+
+    (*here*)
 
     admit.
     admit.
